killing admits related to delta_app_results

steel/Zeta.Steel.ApplicationTypes.fsti
@@ -155,3 +155,16 @@ val spec_result_parser (fid:A.appfn_id aprm)
 
 val spec_result_serializer (fid:A.appfn_id aprm)
   : P.spec_serializer (spec_result_parser fid)
+
+let app_result_entry =
+  (fid:A.appfn_id aprm &
+   app_args fid &
+   app_records fid &
+   app_result fid)
+
+(* A specifiational parser for the arguments of an app function *)
+val spec_app_result_entry_parser
+  : P.spec_parser app_result_entry
+
+val spec_app_result_entry_serializer
+  : P.spec_serializer spec_app_result_entry_parser
